code/experimental/P256/Hacl.Spec.ECDSA.fst
@@ -82,33 +82,16 @@ let _exp_step k i (p, q) =
       _exp_step1 p q 
   else _exp_step0 p q  
 
-val _exp_step_swap : k: scalar -> i: nat {i < 256} -> r0: (tuple2 nat_prime nat_prime) -> Tot
-  (r: tuple2 nat_prime nat_prime
-    {
-      let (p1, q1) = r0 in 
-      let (p2, q2) = r in 
 
-      let (p3, q3) = _exp_step k i r0 in 
-      p2 == p3 /\ q2 == q3
-    }
- )
-      
-  
+val _exponent_spec: k: scalar -> tuple2 nat_prime nat_prime -> Tot (tuple2 nat_prime nat_prime)
 
-let _exp_step_swap k i (p, q) = 
-  let bit = 255 - i in 
-  let bit = ith_bit k bit in 
-  let (p1, q1) = conditional_swap bit p q in 
-  let (p2, q2) = _exp_step1 p1 q1 in 
-  let (p3, q3) = conditional_swap bit p2 q2 in 
-    lemma_swaped_steps p q;
-
-  (p3, q3)  
-  
+let _exponent_spec k (p, q) = 
+  Lib.LoopCombinators.repeati 256  (_exp_step k) (p, q)
 
 
-val exponent_spec: k: scalar -> tuple2 nat_prime nat_prime -> Tot (tuple2 nat_prime nat_prime)
+val exponent_spec: k: scalar -> a: nat_prime -> Tot nat_prime
 
-let exponent_spec k (p, q) = 
-  Lib.LoopCombinators.repeati 256  (_exp_step_swap k) (p, q)
-
+let exponent_spec k a = 
+    let b = 1 in 
+    let a0, _ = _exponent_spec k (1, a) in 
+    a0
